<?xml version="1.0" encoding="UTF-8"?>

<section xml:id="s_der_trig" xmlns:xi="http://www.w3.org/2001/XInclude">
    <title>Derivative: trig functions</title>
    <objectives>
        <ol>
            <li>
                <p>
                    Derive derivative formulas for sine and cosine using the limit definition.
                </p>
            </li>
            <li>
                <p>
                    Derive derivative formulas for tangent, cotangent, secant, and cosecant from the formulas for sine and cosine, using the quotient rule.                     
                </p>
            </li>
            <li>
                <p>
                    Incorporate the new derivative formulas into derivative computations of more complicated functions. 
                </p>
            </li>
        </ol>
    </objectives>
    <theorem xml:id="th_der_sin_cos">
        <title>Derivative formulas: sine and cosine</title>
        <statement>
            <p>
                We have the following derivative formulas: 
                <md>
                    <mrow>\frac{d}{dx}\sin x \amp = \cos x \amp \frac{d}{dx}\cos x\amp =-\sin x</mrow>
                </md>. 
            </p>
        </statement>
        <proof>
            <p>
                We prove the derivative formula for <m>\sin</m>; the argument for <m>\cos</m> is very similar. Using the limit definition of the derivative, we have 
                <md>
                    <mrow>\frac{d}{dx}(\sin x) \amp = \lim\limits_{h\to 0}\frac{\sin(x+h)-\sin x}{h}</mrow>
                    <mrow> \amp \lim\limits_{h\to 0}\frac{\sin x\cos h+\cos x\sin h-\sin x}{h}</mrow>
                    <mrow> \amp = \lim\limits_{h\to 0}\frac{\sin x(\cos h-1)}{h}+\frac{\cos x\sin h}{h}</mrow>
                    <mrow> \amp = \sin x\lim\limits_{h\to 0}\frac{\cos h-1}{h}+\cos x \lim\limits_{h\to 0}\frac{\sin h}{h} </mrow>
                    <mrow> \amp = \sin x\cdot 0 +\cos x\cdot 1</mrow>
                    <mrow> \amp = \cos x</mrow>
                </md>,
                where the penultimate step makes use of our previously discussed limits 
                <md>
                    <mrow>\lim\limits_{t\to 0}\frac{\sin t}{t}  \amp =1 \amp \lim\limits_{t\to 0}\frac{\cos t-1}{t}=0  </mrow>
                </md>.
            </p>
        </proof>
    </theorem>
    <example xml:id="eg_tangent_trig">
    <title>Tangent lines: sinusoidal</title>
    <statement>
    <p>
    Let <m>f(x)=\cos x-\sin x</m>. 
    <ol>
        <li>
            <p>
                Find an equation for the tangent line to the graph of <m>f</m> at <m>x=\pi/3</m>.
            </p>
        </li>
        <li>
            <p>
                Find all points on the graph of <m>f</m> where the tangent line is horizontal. 
            </p>
        </li>
    </ol>
    </p>
    </statement>
    <solution>
    <p>
        <ol>
            <li>
                <p>
                    The tangent line to the graph of <m>f</m> at <m>x=\pi/3</m>, passes through the point 
                    <me>
                        P=(\pi/3, f(\pi/3))=(\pi/3, \cos(\pi/3)-\sin(\pi/3))=(\pi/3, 1/2-\sqrt{3}/2).
                    </me>
                    The slope of the tangent line here is given by <m>f'(\pi/3)</m>. We first compute 
                    <md>
                        <mrow>f'(x) \amp = (\cos x)'-(\sin x)' \amp \text{(lin. comb.)}</mrow>
                        <mrow> \amp = -\sin x-\cos x</mrow>
                    </md>.
                    Thus the slope of the tangent line is 
                    <me>
                        f'(\pi/3)=-\sin(\pi/3)-\cos(\pi/3)=-(\frac{\sqrt{3}+1}{2})
                    </me>,
                    We conclude that an equation for the tangent line here is 
                    <me>
                        y-\frac{1-\sqrt{3}}{2}=-\frac{1+\sqrt{3}}{2}(x-\frac{\pi}{3})
                    </me>. 
                </p>
            </li>
            <li>
                <p>
                    The tangent line to a point <m>P=(x,f(x))</m> on the graph of <m>f</m> is horizontal when its slope <m>f'(x)=0</m>. Thus we need to find all <m>x</m> such that 
                    <me>
                        f'(x)=-\sin x-\cos x=0
                    </me>,
                    or equivalently, 
                    <me>
                        \tan x=-1
                    </me>.
                    The solutions to this trig equation are 
                    <me>
                        x=\frac{3\pi}{4}+\pi n, 
                    </me>
                    where <m>n</m> is an integer. The corresponding points on the graph are 
                    <me>
                        P=\left(\frac{3\pi}{4}+\pi n, f\left(\frac{3\pi}{4}+\pi n\right)\right)
                        = \begin{cases}
                        \left(\frac{3\pi}{4}+\pi n, -\sqrt{2}\right) \amp \text{if } n \text{ is even}\\
                        \left(\frac{3\pi}{4}+\pi n, \sqrt{2}\right) \amp \text{if } n \text{ is odd}\\
                        \end{cases}
                    </me>.
                    
                    
                    
                    
                </p>
            </li>
        </ol>
    </p>
    </solution>
    </example>
    
    <definition xml:id="d_trig_functions">
    <title>Trigonometric functions</title>
    <statement>
    <p>
        We define the <term>tangent</term> (<m>\tan</m>), <term>cotangent</term> (<m>\cot</m>), <term>secant</term> (<m>\sec</m>), and <term>cosecant</term> (<m>\csc</m>) functions as follows:
        <md>
            <mrow>\tan x \amp = \frac{\sin x}{\cos x} \amp \cot x\amp =\frac{\cos x}{\sin x} </mrow>
            <mrow>\sec x \amp =\frac{1}{\cos x} \amp \csc x\amp =\frac{1}{\sin x} </mrow>
        </md>.
    </p>
    </statement>
    </definition>
    <theorem xml:id="th_der_trig">
        <title>Derivative formulas: trig functions</title>
        <statement>
            <p>
               We have the following derivative formulas: 
               <md>
                <mrow>\frac{d}{dx}\sin x \amp = \cos x \amp \frac{d}{dx}\cos x\amp =-\sin x</mrow>
                <mrow>\frac{d}{dx}\tan x \amp = \sec^2 x \amp \frac{d}{dx}\cot x\amp =-\csc^2 x</mrow>
                <mrow>\frac{d}{dx}\sec x \amp = \sec x\tan x \amp \frac{d}{dx}\csc x\amp =-\csc x\cot x</mrow>
               </md>.
            </p>
        </statement>
    </theorem>
    
    
    
    

</section>