<?xml version="1.0" encoding="UTF-8"?>

<section xml:id="s_limit_sandwich" xmlns:xi="http://www.w3.org/2001/XInclude">
    <title>Limits: algebraic technique and sandwich theorem</title>
    <subsection xml:id="ss_alg_tech">
        <title>Algebraic techniques</title>
       <p>
        As we saw in <xref ref="eg_lim_quot_fail"/>, there are limits to usefulness of our limit rules. In many cases, if we run into a dead end, some algebraic manipulation of the function expression can help us find a way forward. The following examples serve to illustrate this technique and remind you of some algebraic techniques. 
       </p> 
       <example>
        <title>Algebraic limit technique: factoring</title>
        <statement>
            <p>
              Compute the limit below. Your answer should be a chain of equalities with steps justified. 

            </p>
        </statement>
        <solution>
            <p>
                
            </p>
        </solution>
       </example>
       <example xml:id="eg_lim_factor">
        <title>Algebraic limit technique: factoring</title>
        <statement>
            <p>
              Compute 
               <me>
                \lim_{v\to 2}\frac{v^3-8}{v^4-16}
               </me>.
               Your answer should be a chain of equalities with steps justified. 
            </p>
        </statement>
        <solution>
            <p>
                Note that the limit of the denominator expression as <m>v\to 2</m> is zero, and thus we cannot directly use the quotient rule. Thus we begin with some algebraic manipulation. The key algebraic technique here is factoring.  
                <md>
                    <mrow>\lim_{v\to 2}\frac{v^3-8}{v^4-16} \amp=\lim_{v\to 2}\frac{(v-2)(v^2+2v+8)}{(v^2-4)(v^2+4)} </mrow>
                    <mrow> \amp = \lim_{v\to 2}\frac{(v-2)(v^2+2v+8)}{(v-2)(v+2)(v^2+4)}</mrow>
                    <mrow> \amp = \lim_{v\to 2}\frac{v^2+2v+8}{(v+2)(v^2+4)} \amp \text{(repl. rule)}</mrow>
                    <mrow> \amp = \frac{2^2+2\cdot 2+8}{(2+2)(2^2+4)} \amp \text{(rational eval.)}</mrow>
                    <mrow> \amp = \frac{16}{32}=\frac{1}{2}</mrow>
                </md>.
            </p>
        </solution>
       </example>
       <example xml:id="eg_limit_clear_denom">
        <title>Algebraic limit technique: clear denominator</title>
        <statement>
            <p>
              Compute  
               <me>
                \lim\limits_{t\to 1}\frac{t-1}{\frac{t^2}{t+2}-\frac{1}{3}}
               </me>.
               Your answer should be a chain of equalities with steps justified.
            </p>
        </statement>
        <solution>
            <p>
               Again, the quotient rule is not available to us, as the limit of the denominator function is zero. Accordingly, we begin with some algebra. 
               <md>
                <mrow>\lim\limits_{t\to 1}\frac{t-1}{\frac{t^2}{t+2}-\frac{1}{3}} \amp =
                    \lim\limits_{t\to 1}\frac{t-1}{\frac{3t^2-t-2}{3(t+2)}} \amp \text{(like denominators)}</mrow>
                <mrow> \amp =\lim\limits_{t\to 1}\frac{3(t-1)(t+2)}{3t^2-t-2}\cdot \frac{3(t+2)}{3(t+2)} </mrow>
                <mrow> \amp =\lim\limits_{t\to 1}\frac{3(t-1)(t+2)}{3t^2-t-2}\cdot \frac{3(t+2)}{3(t+2)} </mrow>
               </md> 
            </p>
        </solution>
       </example>
       <example xml:id="eg_lim_radical">
        <title>Algebraic limit technique: radicals</title>
        <statement>
            <p>
              Compute 
               <me>
                \lim_{x\to 0}\frac{\sqrt{x^2+100}-10}{x^2}
               </me>.
               Your answer should be a chain of equalities with steps justified. 
            </p>
        </statement>
        <solution>
            <p>
               We use the technique of multiplying the numerator and denominator by a <q>conjugate radical</q> expression <m>\sqrt{x^2+100}+10</m>:
               <md>
                <mrow> \lim_{x\to 0}\frac{\sqrt{x^2+100}-10}{x^2}\amp =\lim_{x\to 0}\frac{\sqrt{x^2+100}-10}{x^2}\frac{\sqrt{x^2+100}+10}{\sqrt{x^2+100}+10} \amp \text{(repl. rule)}</mrow>
                <mrow> \amp = \lim_{x\to 0}\frac{x^2+100-10}{x^2(\sqrt{x^2+100}+10)}</mrow>
                <mrow> \amp = \lim_{x\to 0}\frac{1}{\sqrt{x^2+100}+10}</mrow>
                <mrow> \amp = \frac{1}{\sqrt{\lim\limits_{x\to 0}x^2+100}+\lim\limits_{x\to 0}10}
                    \amp \text{(quot., sum, power)}
                </mrow>
                <mrow> \amp = \frac{1}{\sqrt{100}+10} \amp \text{(poly. eval.)}</mrow>
                <mrow> \amp = \frac{1}{20}</mrow>
               </md>.
            </p>
        </solution>
       </example>
    </subsection>
    <subsection xml:id="ss_sandwich">
        <title>Sandwich theorem</title>
        <p>
            Another situation where our basic limit rules might not suffice to compute a given limit is when the function <m>f</m> in question is unreasonably complicated, making its behavior near a point difficult to pin down. The <xref ref="th_sandwich" text="custom">sandwich theorem</xref> potentially gives a technique for getting around this issue. You can think of it as a means of replacing the complicated function <m>f</m>, whose behavior is a mystery to us, with two simpler <q>bounding</q> functions <m>g</m> and <m>h</m>, whose behavior we understand. It is called the sandwich theorem as the necessary inequality <m>g(x)\leq f(x)\leq h(x)</m> has <m>f</m> <q>sandwiched</q> between the functions <m>g</m> and <m>h</m>.   
        </p>
        <theorem xml:id="th_sandwich">
            <title>Sandwich theorem</title>
            <statement>
                <p>
                Fix a point <m>a\in \R</m> and suppose that functions <m>f,g,h</m> satisfy <m>g(x)\leq f(x)\leq h(x)</m> for all <m>x\ne a</m> lying in an open interval containing <m>a</m>. If 
                <me>
                    \lim_{x\to a}g(x)=\lim_{x\to a}h(x)=L
                </me>,
                then
                <me>
                    \lim_{x\to a}f(x)=L
                </me>.
                Using logical shorthand: 
                <md>
                    <mrow>\left(g(x)\leq f(x)\leq h(x) \text{ and }  \lim_{x\to a}g(x)=\lim_{x\to a}h(x)=L\right)\amp\implies \lim_{x\to a}f(x)=L </mrow>
                </md>.
                </p>
            </statement>
            <proof>
                <p>
                    As with all bits of theory in mathematics, this statement requires proof; and as with most bits of theory in this course, we will not provide that proof. Interested in seeing how one would prove this and other statements from calculus? Take Math 320-1 or Math 321-1! 
                </p>
            </proof>
        </theorem>
        <p>
            Making use of the sandwich theorem requires carrying out a number of steps (with justification). The following procedure will be useful for doing this in an organized manner. 
        </p>
        <algorithm xml:id="proc_sandwich">
            <title>Sandwich theorem</title>
            <statement>
                <p>
                    To compute <m>\lim_{x\to a}f(x)</m> using the sandwich theorem, proceed as follows. 
                    <ol>
                        <li>
                            <p>
                                Find bounding functions <m>g</m> and <m>h</m> satisfying the two following conditions: 
                                <ol>
                                    <li>
                                        <p>
                                            <m>g(x)\leq f(x)\leq h(x)</m> for all <m>x\ne a</m> lying in an open interval containing <m>a</m>.
                                        </p>
                                    </li>
                                    <li>
                                        <p>
                                            <m>\lim\limits_{x\to a}g(x)=\lim\limits_{x\to a}h(x)=L</m> for some <m>L\in \R</m>. 
                                        </p>
                                    </li>
                                </ol>
                            For your own convenience, make sure to <em>name</em> these functions, as opposed to just providing formulas for them. 
                            </p>
                        </li>
                        <li>
                            <p>
                                Conclude (citing the sandwich theorem) that <m>\lim\limits_{x\to a}f(x)=L</m>
                            </p>
                        </li>
                    </ol>
                </p>
            </statement>
        </algorithm>
    <remark xml:id="rm_sandwich">
        <title>Sandwich theorem</title>
        <p>
        As the examples below will illustrate, the art of using <xref ref="proc_sandwich"/> lies in being able to find <em>useful</em> bounding functions <m>g</m> and <m>h</m>.  Use these examples as a model for your own use of <xref ref="proc_sandwich"/>. Note in particular how 
        <ul>
            <li>
                <p>
                    the explanations make explicit the two conditions that the bounding functions must satisfy;
                </p>
            </li>
            <li>
                <p>
                    the explanations end with a concluding statement explicitly citing the sandwich theorem;
                </p>
            </li>
            <li>
                <p>
                    giving the bounding functions <em>names</em> (<eg/>, <m>g</m> and <m>h</m>), as opposed to just providing formulas (<eg/>, <m>1-x^2/4</m>, <m>1+x^2/4</m>), makes these explanations more concise. 
                </p>
            </li>
        </ul>
    </p></remark>
    <example xml:id="eg_sandwich_easy">
        <title>Sandwich theorem: easy</title>
        <statement>
            <p>
                Suppose the function <m>f(x)</m> satisfies 
                <me>
                    1-\frac{x^2}{4}\leq f(x)\leq 1+\frac{x^2}{4}
                </me>
                for all <m>x\ne 0</m> in the interval <m>(-1/3, 1/3)</m>. Compute <m>\lim_{x\to 0}f(x)</m>. 
            </p>
        </statement>
        <solution>
            <p>
            We follow the steps of <xref ref="proc_sandwich"/>. In this case our bounding functions <m>g(x)=1-x^2/4</m> and <m>h(x)=1+x^2/4</m> are provided for us, making life much easier. By assumption our mystery function <m>f</m> satisfies 
            <men xml:id="eq_sand_easy">
                g(x)\leq f(x)\leq h(x)
            </men>
            for all <m>x\ne 0\in (-1/3, 1/3)</m>. Next we compute 
            <md>
                <mrow>\lim_{x\to 0}g(x) \amp = 1-0^2/4 \amp \text{(poly. eval.)}</mrow>
                <mrow> \amp =1</mrow>
                <mrow>\lim_{x\to 0}h(x) \amp = 1+0^2/4 \amp \text{(poly. eval.)}</mrow>
                <mrow> \amp =1</mrow>
            </md>.
            Since <xref ref="eq_sand_easy"/> holds for all <m>x\ne 0\in (-1/3,1/3)</m>, and since 
            <me>
                \lim_{x\to 0}g(x)=\lim_{x\to 0}h(x)=1
            </me>,
            we conclude that <m>\lim\limits_{x\to 0}f(x)=1</m>. 
            

            
            </p>
        </solution>
    </example>
    <example xml:base="eg_sandwich_harder">
        <title>Sandwich theorem: harder</title>
        <statement>
            <p>
                Use the sandwich theorem to compute <m>\lim\limits_{x\to 0}x^2\cos(1/x)</m>.
            </p>
        </statement>
        <solution>
            <p>
                
            </p>
        </solution>
    </example>
    </subsection>

</section>